verifies with blood objects

projectVampire/dafny/insertionSort.dfy
@@ -1,36 +1,215 @@
+// state:
+// unsafe = -1
+// unverified = 0
+// verified = 1
+// storage = 2
+// dispatch = 3
+// delivered = 4
+
+datatype Blood_types = O | A | B | AB
+
+class Blood{
+    var state: int;
+    var collection_time: int; //Seconds since Unix Epoch
+    var expiry_time:int
+    var blood_type: Blood_types;
+    var rhesus: bool;
+
+    predicate method Valid()
+    reads this
+    {-1<=state<=4}
+
+    predicate method expired(curr_time:int)
+    reads this
+    {curr_time>expiry_time}
+
+    predicate method safe(curr_time:int)
+    reads this
+    {0<=state<=4 && !expired(curr_time)}
+
+    constructor (secondsin:int)
+    modifies this
+    requires secondsin>=0
+    ensures collection_time>=0 && collection_time==secondsin
+    ensures state == 0;
+    {
+        collection_time := secondsin;
+        expiry_time:=collection_time;
+        state := 0;
+    }
+
+    method verify(curr_time:int,determined_type:Blood_types,rhesus_in:bool)
+    modifies this;
+    requires state==0;
+    ensures if safe(curr_time) then state ==1 else state==-1
+    ensures blood_type==determined_type
+    ensures rhesus == rhesus_in
+    {
+        if safe(curr_time) {
+            state:=1;
+        } else {
+            state:=-1;
+        }
+    blood_type:=determined_type;
+    rhesus:=rhesus_in;
+    }
+
+    method store(curr_time:int)
+    modifies this
+    requires state==1;
+    ensures if safe(curr_time) then state ==2 else state==-1;
+    {
+        if safe(curr_time) {
+            state:=2;
+        } else {
+            state:=-1;
+        }  
+    }
+
+    method dispatch(curr_time:int)
+    modifies this
+    requires state==2;
+    ensures if safe(curr_time) then state ==3 else state==-1;
+    {
+        if safe(curr_time) {
+            state:=3;
+        } else {
+            state:=-1;
+        }         
+    }
+
+    method delivered(curr_time:int)
+    modifies this
+    requires state==3;
+    ensures if safe(curr_time) then state ==4 else state==-1;
+    {
+        if safe(curr_time) {
+            state:=4;
+        } else {
+            state:=-1;
+        }           
+    }
+
+    method reject()
+    modifies this
+    ensures state ==-1;
+    {state:=-1;}
+}
+
+
 predicate Sorted(arr: array<int>, start:int, end:int)
 requires arr != null;
 requires 0<=start<arr.Length;
 requires end <= arr.Length;
+//requires forall x :: 0 <= x < arr.Length ==> arr[x] != null;
 reads arr;
 {
     forall i, j :: start <= i < j < end ==> arr[i] <= arr[j]
 }
 
 
-method insertionSort(toSort: array<int>)
+
+// Expiry time and values in two arrays match
+predicate Matching(arr1: array<int>, arr2: array<Blood>)
+requires arr1 != null;
+requires arr2 != null;
+requires arr1.Length == arr2.Length;
+reads arr1;
+reads arr2;
+reads arr2[..];
+{
+	forall i :: 0 <= i < arr1.Length && arr2[i] != null ==> arr2[i].expiry_time == arr1[i]
+}
+
+
+//method bloodSort(toSort: array<Blood>, sortedArray: array<int>) returns (sortedBlood: array<Blood>)
+//modifies toSort;
+//requires toSort != null;
+//requires sortedArray != null;
+//requires forall x :: exists y :: 0 <= x < toSort.Length && 0 <= y < sortedArray.Length && toSort[x] != null && toSort[x].expiry_time == sortedArray[y] // requires mapping from sorted to toSort
+//requires toSort.Length == sortedArray.Length;
+//ensures sortedBlood != null;
+//ensures toSort.Length == sortedBlood.Length;
+//ensures forall x :: 0 <= x < sortedBlood.Length && sortedBlood[x] != null ==> sortedBlood[x].expiry_time == sortedArray[x]; // a mapping between sorted array an blood expiry
+//{
+//	var x := 0;
+//	var y := 0;
+//	sortedBlood := new Blood[toSort.Length]; 
+//	while x < toSort.Length 
+//	invariant 0 <= x <= toSort.Length
+//	//invariant forall i :: 0 <= i < x ==> sortedBlood[i] != null
+//	//invariant forall i :: 0 <= i < x  && sortedBlood[i] != null==> sortedBlood[i].expiry_time == sortedArray[i]
+//	{
+//		 
+//		y := 0;
+//		while y < toSort.Length 
+//			invariant 0 <= y <= toSort.Length
+//			//invariant forall i :: 0 <= i < y && toSort[i] != null && sortedBlood[i] != null && sortedBlood[i] == toSort[x] ==> i == y
+//			//invariant exists i :: 0 <= i < (y-1) && toSort[i] != null && toSort[i].expiry_time == sortedArray[i]
+//			{
+//			if (toSort[y] != null && sortedArray[x] == toSort[y].expiry_time) {
+//				sortedBlood[x] := toSort[x];
+//				toSort[y] := null; // so we don't capture this object again
+//			}
+//			y := y + 1;
+//		}	 
+//		x := x + 1;
+//	}
+//}
+
+
+
+
+
+
+
+
+method insertionSort(toSort: array<int>, toMatch: array<Blood>)
 requires toSort != null;
+requires toMatch != null;
+requires toSort.Length == toMatch.Length;
+//requires forall x :: 0 <= x < toSort.Length ==> toSort[x] != null
+requires forall x,y ::0 <= x < toSort.Length && 0 <= y < toMatch.Length && x == y  && toMatch[y] != null ==> toMatch[y].expiry_time == toSort[x];
+
 requires toSort.Length > 1;
 ensures Sorted(toSort,0,toSort.Length-1);
 ensures multiset(toSort[..]) == multiset(old(toSort[..]));
+ensures forall x, y :: 0 <= x < toSort.Length && 0 <= y < toMatch.Length && x == y && toMatch[y] != null ==> toMatch[y].expiry_time == toSort[x];
 modifies toSort;
+modifies toMatch;
 {
     var start := 1;
     while (start < toSort.Length)
     invariant 1 <= start <= toSort.Length;
     invariant Sorted(toSort, 0, start); // array is sorted up to start
     invariant multiset(toSort[..]) == multiset(old(toSort[..])); // keep array the same
+    invariant multiset(toMatch[..]) == multiset(old(toMatch[..]));
+    invariant forall x, y :: 0 <= x < toMatch.Length && 0 <= toSort.Length && x == y && toMatch[x] != null ==> toSort[y] == toMatch[x].expiry_time;
+    //invariant Matching(toSort, toMatch);
+    //invariant forall x :: 0 <= x < toSort.Length ==> toSort[x] != null
+    //invariant forall x :: 0 <= x < toSort.Length 
     {
         var end := start;
         while (end >= 1 && toSort[end-1] > toSort[end])
         invariant 0 <= end <= start; // end is within limits
         invariant multiset(toSort[..]) == multiset(old(toSort[..])); // array stays the same
+	invariant multiset(toMatch[..]) == multiset(old(toMatch[..]));
+	//invariant Matching(toSort, toMatch);
+	//invariant forall i :: 0 <= i < toSort.Length ==> toSort[i] != null;
         invariant forall i, j :: (0 <= i <= j <= start && j != end) ==> toSort[i] <= toSort[j]; // all values less than start are sorted
-        {
-            var temp := toSort[end-1];
-            toSort[end-1] := toSort[end];
-            toSort[end] := temp;
-            end := end - 1;
+        //invariant forall i :: (0 <= i <= start && i != end && toMatch[i] != null) ==> toSort[i] == toMatch[i].expiry_time;
+        invariant forall x, y :: 0 <= x < toMatch.Length && 0 <= toSort.Length && x == y && toMatch[x] != null ==> toSort[y] == toMatch[x].expiry_time;
+	{
+           	var temp := toSort[end-1];
+           	toSort[end-1] := toSort[end];
+            	toSort[end] := temp;
+		
+	    	var temp2 := toMatch[end-1];
+	    	toMatch[end-1] := toMatch[end];
+	    	toMatch[end] := temp2;
+		
+		end := end -1;
+		
         }
         start := start + 1;
     }
@@ -39,13 +218,27 @@ modifies toSort;
 
 method Test()
 {
-    var test1 := new int[4];
-    test1[0] := 10;
-    test1[1] := 5;
-    test1[2] := 12;
-    test1[3] := 1;
+    var nums := new int[3];
+    //nums[0] := 10;
+    //nums[1] := 5;
+    //nums[2] := 1;
     
-    insertionSort(test1);
-    assert Sorted(test1,0,test1.Length-1);    
+    var blood := new Blood[3];
+    var temp := new Blood(10);
+    blood[0] := temp; 
+    temp := new Blood(5);
+    blood[1] := temp;
+    temp := new Blood(1);
+    blood[2] := temp;
+   
+    nums[0] := blood[0].expiry_time;
+    nums[1] := blood[1].expiry_time;
+    nums[2] := blood[2].expiry_time; 
 
+    assert nums.Length == blood.Length;
+    assert forall x,y ::0 <= x < nums.Length &&  0 <= y < blood.Length && x == y ==> nums[x] == blood[y].expiry_time; 
+    insertionSort(nums, blood);
+    assert Sorted(nums,0,nums.Length-1); // array is sorted and blood has maintained 1-1 correspondence with the now sorted array
+    assert forall x, y :: 0 <= x < nums.Length && 0 <= y < blood.Length && x == y && blood[y] != null ==> nums[x] == blood[y].expiry_time;    
 }
+
